proof/access-control/Arch_AC.thy
@@ -252,7 +252,8 @@ where
        pas_cap_cur_auth aag cap \<and> is_subject aag (fst ptr) \<and> authorised_slots aag slots
    | ArchInvocation_A.PageRemap asid slots \<Rightarrow> authorised_slots aag slots
    | ArchInvocation_A.PageUnmap cap ptr \<Rightarrow> pas_cap_cur_auth aag (Structures_A.ArchObjectCap cap) \<and> is_subject aag (fst ptr)
-   | ArchInvocation_A.PageFlush typ start end pstart pd asid \<Rightarrow> True"
+   | ArchInvocation_A.PageFlush typ start end pstart pd asid \<Rightarrow> True
+   | ArchInvocation_A.PageGetAddr ptr \<Rightarrow> True"
 
 crunch respects[wp]: check_mapping_pptr "integrity X aag st"
 
@@ -487,8 +488,132 @@ lemma invalidate_tlb_by_asid_pas_refined[wp]:
   "\<lbrace>pas_refined aag\<rbrace> invalidate_tlb_by_asid asid \<lbrace>\<lambda>rv. pas_refined aag\<rbrace>"
   by (wp dmo_no_mem_respects | wpc | simp add: invalidate_tlb_by_asid_def invalidateTLB_ASID_def)+
 
+crunch pas_refined[wp]: set_message_info "pas_refined aag"
+
+(* FIXME: move *)
+lemma set_message_info_mdb[wp]:
+  "\<lbrace>\<lambda>s. P (cdt s)\<rbrace> set_message_info thread info \<lbrace>\<lambda>rv s. P (cdt s)\<rbrace>"
+  unfolding set_message_info_def by wp
+
+crunch state_vrefs[wp]: do_machine_op "\<lambda>s::'z::state_ext state. P (state_vrefs s)"
+
+crunch thread_states[wp]: do_machine_op "\<lambda>s. P (thread_states s)"
+
+(* FIXME: move *)
+lemma set_mrs_state_vrefs[wp]:
+  "\<lbrace>\<lambda>s. P (state_vrefs s)\<rbrace> set_mrs thread buf msgs \<lbrace>\<lambda>rv s. P (state_vrefs s)\<rbrace>"
+  apply (simp add: set_mrs_def split_def set_object_def)
+  apply (wp gets_the_wp get_wp put_wp mapM_x_wp'
+       | wpc
+       | simp split del: split_if add: zipWithM_x_mapM_x split_def store_word_offs_def)+
+  apply (auto simp: obj_at_def state_vrefs_def get_tcb_ko_at
+             elim!: rsubst[where P=P, OF _ ext]
+             split: split_if_asm simp: vs_refs_no_global_pts_def)
+  done
+
+(* FIXME: move *)
+lemma set_mrs_thread_states[wp]:
+  "\<lbrace>\<lambda>s. P (thread_states s)\<rbrace> set_mrs thread buf msgs \<lbrace>\<lambda>rv s. P (thread_states s)\<rbrace>"
+  apply (simp add: set_mrs_def split_def set_object_def)
+  apply (wp gets_the_wp get_wp put_wp mapM_x_wp'
+       | wpc
+       | simp split del: split_if add: zipWithM_x_mapM_x split_def store_word_offs_def)+
+  apply (clarsimp simp: fun_upd_def[symmetric] thread_states_preserved)
+  done
+
+lemma set_mrs_pas_refined[wp]:
+  "\<lbrace>pas_refined aag\<rbrace> set_mrs thread buf msgs \<lbrace>\<lambda>rv. pas_refined aag\<rbrace>"
+  apply (simp add: pas_refined_def state_objs_to_policy_def)
+  apply (rule hoare_pre)
+   apply (wp | wps)+
+  apply (clarsimp dest!: auth_graph_map_memD)
+  done
+
+crunch integrity_autarch: set_message_info "integrity aag X st"
+
+lemma storeWord_respects:
+  "\<lbrace>\<lambda>ms. integrity aag X st (s\<lparr>machine_state := ms\<rparr>) \<and> (\<forall>p' \<in> ptr_range p 2. aag_has_auth_to aag Write p')\<rbrace> storeWord p v \<lbrace>\<lambda>a b. integrity aag X st (s\<lparr>machine_state := b\<rparr>)\<rbrace>"
+  unfolding storeWord_def
+  apply wp
+  apply (auto simp: integrity_def is_aligned_mask [symmetric] intro!: trm_write ptr_range_memI ptr_range_add_memI)
+  done
+
+lemma dmo_storeWord_respects_Write:
+  "\<lbrace>integrity aag X st and K (\<forall>p' \<in> ptr_range p 2. aag_has_auth_to aag Write p')\<rbrace> 
+  do_machine_op (storeWord p v)
+  \<lbrace>\<lambda>a. integrity aag X st\<rbrace>"
+  apply (rule hoare_pre)
+  apply (wp dmo_wp storeWord_respects)
+  apply simp
+  done
+
+(* c.f.  auth_ipc_buffers *)
+definition
+  ipc_buffer_has_auth :: "'a PAS \<Rightarrow> word32 \<Rightarrow> word32 option \<Rightarrow> bool"
+where
+   "ipc_buffer_has_auth aag thread \<equiv> 
+    option_case True (\<lambda>buf'. is_aligned buf' msg_align_bits \<and> (\<forall>x \<in> ptr_range buf' msg_align_bits. (pasObjectAbs aag thread, Write, pasObjectAbs aag x) \<in> pasPolicy aag))"
+
+lemma ipc_buffer_has_auth_wordE:
+  "\<lbrakk> ipc_buffer_has_auth aag thread (Some buf); p \<in> ptr_range (buf + off) sz; is_aligned off sz; sz \<le> msg_align_bits; off < 2 ^ msg_align_bits \<rbrakk> 
+  \<Longrightarrow> (pasObjectAbs aag thread, Write, pasObjectAbs aag p) \<in> pasPolicy aag"
+  unfolding ipc_buffer_has_auth_def
+  apply clarsimp
+  apply (erule bspec)
+  apply (erule (4) set_mp [OF ptr_range_subset])
+  done
+
+
+lemma is_aligned_word_size_2 [simp]:
+  "is_aligned (p * of_nat word_size) 2"
+  unfolding word_size_def 
+  by (simp add: is_aligned_mult_triv2 [where n = 2, simplified] word_bits_conv)
+
+
+
+lemma mul_word_size_lt_msg_align_bits_ofnat:
+  "p < 2 ^ (msg_align_bits - 2) \<Longrightarrow> of_nat p * of_nat word_size < (2 :: word32) ^ msg_align_bits"
+  unfolding word_size_def
+  apply simp
+  apply (rule word_less_power_trans_ofnat [where k = 2, simplified])
+  apply (simp_all add: msg_align_bits word_bits_conv)
+  done
+
+lemma store_word_offs_integrity_autarch:
+  "\<lbrace>integrity aag X st and K (is_subject aag thread \<and> ipc_buffer_has_auth aag thread (Some buf) \<and> r < 2 ^ (msg_align_bits - 2))\<rbrace>
+   store_word_offs buf r v
+   \<lbrace>\<lambda>rv. integrity aag X st\<rbrace>"
+  apply (simp add: store_word_offs_def)
+  apply (rule hoare_pre)
+   apply (wp dmo_storeWord_respects_Write)
+  apply clarsimp
+  apply (drule (1) ipc_buffer_has_auth_wordE)
+     apply simp
+    apply (simp add: msg_align_bits)
+   apply (erule mul_word_size_lt_msg_align_bits_ofnat)
+  apply simp
+  done
+
+lemma set_mrs_integrity_autarch:
+  "\<lbrace>integrity aag X st and K (is_subject aag thread \<and>  ipc_buffer_has_auth aag thread buf)\<rbrace>
+     set_mrs thread buf msgs
+   \<lbrace>\<lambda>rv. integrity aag X st\<rbrace>"
+  apply (rule hoare_gen_asm)
+  apply (simp add: set_mrs_def)
+  apply (wp gets_the_wp get_wp put_wp mapM_x_wp' store_word_offs_integrity_autarch [where aag = aag and thread = thread]
+       | wpc
+       | simp split del: split_if add: split_def zipWithM_x_mapM_x )+
+    apply (clarsimp elim!: in_set_zipE split: split_if_asm)
+    apply (rule order_le_less_trans [where y = msg_max_length])
+     apply (fastforce simp add: le_eq_less_or_eq)
+    apply (simp add: msg_max_length_def msg_align_bits)
+   apply simp
+   apply (wp set_object_integrity_autarch hoare_drop_imps hoare_vcg_all_lift)
+  apply simp
+  done
+
 lemma perform_page_invocation_respects:
-  "\<lbrace>integrity aag X st and pas_refined aag and K (authorised_page_inv aag pi) and valid_page_inv pi and valid_arch_objs and pspace_aligned\<rbrace>
+  "\<lbrace>integrity aag X st and pas_refined aag and K (authorised_page_inv aag pi) and valid_page_inv pi and valid_arch_objs and pspace_aligned and is_subject aag  \<circ> cur_thread\<rbrace>
      perform_page_invocation pi
    \<lbrace>\<lambda>s. integrity aag X st\<rbrace>"
 proof -
@@ -520,7 +645,7 @@ proof -
    apply (drule (1) clas_caps_of_state)
    apply (simp add: cap_links_asid_slot_def label_owns_asid_slot_def)
    apply (auto dest: pas_refined_Control)[1]
-  apply (wp | simp)+
+  apply (wp set_mrs_integrity_autarch set_message_info_integrity_autarch | simp add: ipc_buffer_has_auth_def)+
   done
 qed
 
@@ -556,7 +681,6 @@ lemma perform_page_invocation_pas_refined [wp]:
                           cap_auth_conferred_def vspace_cap_rights_to_auth_def
                           cli_no_irqs is_pg_cap_def pte_ref_def
                           [simplified aag_cap_auth_def])+
-  apply clarsimp
   done
 
 definition
@@ -890,7 +1014,7 @@ crunch respects [wp]: perform_page_directory_invocation "integrity aag X st"
   (ignore: do_machine_op)
 
 lemma invoke_arch_respects:
-  "\<lbrace>integrity aag X st and K (authorised_arch_inv aag ai) and pas_refined aag and invs and valid_arch_inv ai\<rbrace>
+  "\<lbrace>integrity aag X st and K (authorised_arch_inv aag ai) and pas_refined aag and invs and valid_arch_inv ai and is_subject aag \<circ> cur_thread\<rbrace>
      arch_perform_invocation ai
    \<lbrace>\<lambda>s. integrity aag X st\<rbrace>"
   apply (simp add: arch_perform_invocation_def)
