proof/invariant-abstract/EmptyFail_AI.thy
@@ -333,7 +333,7 @@ lemma arch_decode_ARMASIDPoolAssign_empty_fail:
 lemma arch_decode_invocation_empty_fail[wp]:
   "empty_fail (arch_decode_invocation label b c d e f)"
   apply (case_tac "invocation_type label")
-                                  apply ((simp add: arch_decode_invocation_def Let_def split: arch_cap.splits cap.splits option.splits | wp | intro conjI impI allI)+)[39]
+                                  apply ((simp add: arch_decode_invocation_def Let_def split: arch_cap.splits cap.splits option.splits | wp | intro conjI impI allI)+)[40]
    apply (simp add: arch_decode_ARMASIDControlMakePool_empty_fail arch_decode_ARMASIDPoolAssign_empty_fail)+
    done
 
